KrakenAArch64.lean
@@ -6,3 +6,5 @@
 
 import Kraken.AArch64.Semantics
 import Kraken.AArch64.Parser
+import Kraken.AArch64.OmniSemantics
+import Kraken.AArch64.Examples.SumToN
